Chain proof owner never changes

examples/fac_master/piggybank/PiggyBank.v
@@ -29,6 +29,8 @@ Section PiggyBank.
                   owner : Address ; 
                   piggyState : PiggyState}.
 
+  Definition Setup : Type := unit.
+
   Definition insert (n : Amount) (st : State) : State :=
       {| balance := st.(balance) + n ;
           owner := st.(owner);
@@ -66,7 +68,7 @@ Section PiggyBank.
        end.
 
   (** We initialize the contract state with [init_value] and set [owner] to the address from which the contract was deployed *)
-  Definition piggyBank_init (chain : Chain) (ctx : ContractCallContext) (_ : Amount) : option State :=
+  Definition piggyBank_init (chain : Chain) (ctx : ContractCallContext) (_ : Setup) : option State :=
   Some {| balance := 0 ;
           owner := ctx.(ctx_from);
           piggyState := Intact |}.
@@ -82,7 +84,7 @@ Section PiggyBank.
     Derive Serializable Msg_rect<Insert, Smash>.
 
   (** The piggybank contract *)
-  Definition piggyBank_contract : Contract Amount Msg State :=
+  Definition piggyBank_contract : Contract Setup Msg State :=
     build_contract piggyBank_init piggyBank_receive.
 
 End PiggyBank.
@@ -169,5 +171,33 @@ Section SafetyProperties.
     inversion H0. cbn in *. apply Z.ltb_lt in H1. omega.
     + destruct cstate, piggyState0; try easy. destruct (address_eqb ctx.(ctx_from) owner0); try easy.
     inversion H0. cbn in *. easy.
-  Qed. 
+  Qed.
+
+  Lemma owner_never_changes2 : forall bstate caddr (trace : ChainTrace empty_state bstate),
+    reachable bstate ->
+    env_contracts bstate caddr = Some (piggyBank_contract : WeakContract) ->
+    exists cstate depinfo,
+      contract_state bstate caddr = Some cstate /\
+      deployment_info Setup trace caddr = Some depinfo /\
+      depinfo.(deployment_from) = cstate.(owner).
+  Proof.
+    contract_induction;
+      intros; auto.
+      - cbn in *. unfold piggyBank_init in init_some. inversion init_some. easy.
+      - cbn in *. unfold piggyBank_receive in receive_some. destruct msg; try easy.
+        unfold piggyBank in receive_some. destruct m; try easy. destruct (0 <? ctx_amount ctx); try easy.
+        + rewrite IH. destruct prev_state. cbn in *. destruct piggyState0; try easy. inversion receive_some. easy.
+        + rewrite IH. destruct prev_state. cbn in *. destruct piggyState0; try easy. destruct_address_eq; try easy.
+        inversion receive_some. easy.
+      - rewrite IH. cbn in *. unfold piggyBank_receive in receive_some. destruct msg; try easy.
+        unfold piggyBank in receive_some. destruct m.
+        + destruct (0 <? ctx_amount ctx); try easy. destruct prev_state. destruct piggyState0; try easy. inversion receive_some. easy.
+        + destruct prev_state. destruct piggyState0; try easy. destruct_address_eq; try easy. inversion receive_some. easy.
+      - instantiate (AddBlockFacts := fun _ _ _ _ _ _ => True).
+        instantiate (DeployFacts := fun _ _ => True).
+        instantiate (CallFacts := fun _ _ _ _ => True).
+        unset_all; subst;cbn in *.
+        destruct_chain_step; auto.
+        destruct_action_eval; auto.
+  Qed.
 End SafetyProperties.
